Weidenbach_Book/Watched_Literals_List_Restart.thy
@@ -2855,6 +2855,7 @@ qed
 definition cdcl_twl_stgy_restart_abs_early_l :: "'v twl_st_l \<Rightarrow> 'v twl_st_l nres" where
   \<open>cdcl_twl_stgy_restart_abs_early_l S\<^sub>0 =
   do {
+    ebrk \<leftarrow> RES UNIV;
     (_, brk, T, n) \<leftarrow> WHILE\<^sub>T\<^bsup>\<lambda>(ebrk, brk, T, n). cdcl_twl_stgy_restart_abs_l_inv S\<^sub>0 brk T n\<^esup>
       (\<lambda>(ebrk, brk, _). \<not>brk \<and> \<not>ebrk)
       (\<lambda>(_, brk, S, n).
@@ -2865,7 +2866,7 @@ definition cdcl_twl_stgy_restart_abs_early_l :: "'v twl_st_l \<Rightarrow> 'v tw
 	ebrk \<leftarrow> RES UNIV;
         RETURN (ebrk, brk, T, n)
       })
-      (False, False, S\<^sub>0, 0);
+      (ebrk, False, S\<^sub>0, 0);
     if \<not>brk then do {
       (brk, T, _) \<leftarrow> WHILE\<^sub>T\<^bsup>\<lambda>(brk, T, n). cdcl_twl_stgy_restart_abs_l_inv S\<^sub>0 brk T n\<^esup>
       (\<lambda>(brk, _). \<not>brk)
@@ -2880,10 +2881,28 @@ definition cdcl_twl_stgy_restart_abs_early_l :: "'v twl_st_l \<Rightarrow> 'v tw
       RETURN T
     } else RETURN T
   }\<close>
-  
+
+definition cdcl_twl_stgy_restart_prog_l :: "'v twl_st_l \<Rightarrow> 'v twl_st_l nres" where
+  \<open>cdcl_twl_stgy_restart_prog_l S\<^sub>0 =
+  do {
+    (brk, T, n) \<leftarrow> WHILE\<^sub>T\<^bsup>\<lambda>(brk, T, n). cdcl_twl_stgy_restart_abs_l_inv S\<^sub>0 brk T n\<^esup>
+      (\<lambda>(brk, _). \<not>brk)
+      (\<lambda>(brk, S, n).
+      do {
+	T \<leftarrow> unit_propagation_outer_loop_l S;
+	(brk, T) \<leftarrow> cdcl_twl_o_prog_l T;
+	(T, n) \<leftarrow> restart_prog_l T n brk;
+	RETURN (brk, T, n)
+      })
+      (False, S\<^sub>0, 0);
+    RETURN T
+  }\<close>
+
+
 definition cdcl_twl_stgy_restart_prog_early_l :: "'v twl_st_l \<Rightarrow> 'v twl_st_l nres" where
   \<open>cdcl_twl_stgy_restart_prog_early_l S\<^sub>0 =
   do {
+    ebrk \<leftarrow> RES UNIV;
     (ebrk, brk, T, n) \<leftarrow> WHILE\<^sub>T\<^bsup>\<lambda>(ebrk, brk, T, n). cdcl_twl_stgy_restart_abs_l_inv S\<^sub>0 brk T n\<^esup>
       (\<lambda>(ebrk, brk, _). \<not>brk \<and> \<not>ebrk)
       (\<lambda>(ebrk, brk, S, n).
@@ -2894,7 +2913,7 @@ definition cdcl_twl_stgy_restart_prog_early_l :: "'v twl_st_l \<Rightarrow> 'v t
 	ebrk \<leftarrow> RES UNIV;
         RETURN (ebrk, brk, T, n)
       })
-      (False, False, S\<^sub>0, 0);
+      (ebrk, False, S\<^sub>0, 0);
     if \<not>brk then do {
       (brk, T, n) \<leftarrow> WHILE\<^sub>T\<^bsup>\<lambda>(brk, T, n). cdcl_twl_stgy_restart_abs_l_inv S\<^sub>0 brk T n\<^esup>
 	(\<lambda>(brk, _). \<not>brk)
@@ -2983,7 +3002,7 @@ lemma cdcl_twl_stgy_restart_abs_early_l_cdcl_twl_stgy_restart_abs_early_l:
       cdcl_twl_o_prog_l_spec[THEN fref_to_Down]
       restart_abs_l_restart_prog[THEN fref_to_Down_curry2])
   subgoal by simp
-  subgoal for x y xa x' x1 x2 x1a x2a
+  subgoal for x y _ _ xa x' x1 x2 x1a x2a
     unfolding cdcl_twl_stgy_restart_abs_l_inv_def
     apply (rule_tac x=y in exI)
     apply (rule_tac x=\<open>fst (snd (snd x'))\<close> in exI)
@@ -3000,7 +3019,7 @@ lemma cdcl_twl_stgy_restart_abs_early_l_cdcl_twl_stgy_restart_abs_early_l:
   subgoal by auto
   subgoal by auto
   subgoal by auto
-  subgoal for x y xa x' x1 x2 x1a x2a x1b x2b x1c x2c x1d x2d x1e x2e xb x'a x1f x2f x1g
+  subgoal for x y _ _ xa x' x1 x2 x1a x2a x1b x2b x1c x2c x1d x2d x1e x2e xb x'a x1f x2f x1g
     unfolding cdcl_twl_stgy_restart_abs_l_inv_def
     apply (rule_tac x=y in exI)
     apply (rule_tac x=\<open>fst (snd x'a)\<close> in exI)
@@ -3031,6 +3050,96 @@ lemma (in twl_restart) cdcl_twl_stgy_restart_prog_early_l_cdcl_twl_stgy_restart_
     apply fast
     apply assumption
   apply (rule cdcl_twl_stgy_restart_prog_early_l_cdcl_twl_stgy_restart_abs_early_l[THEN fref_to_Down,
+    simplified])
+  apply simp
+  done
+
+lemma cdcl_twl_stgy_restart_prog_l_cdcl_twl_stgy_restart_abs_l:
+  \<open>(cdcl_twl_stgy_restart_prog_l, cdcl_twl_stgy_restart_abs_l) \<in> {(S, S').
+   (S, S') \<in> Id \<and>  twl_list_invs S \<and>  clauses_to_update_l S =  {#}} \<rightarrow>\<^sub>f \<langle>Id\<rangle> nres_rel\<close>
+   (is \<open>_ \<in> ?R \<rightarrow>\<^sub>f _\<close>)
+proof -
+  have [refine0]: \<open>((False, S, 0), (False, T , 0)) \<in> bool_rel \<times>\<^sub>r ?R \<times>\<^sub>r nat_rel\<close>
+    if \<open>(S, T) \<in> ?R\<close>
+    for S T
+    using that by auto
+  have [refine0]: \<open>unit_propagation_outer_loop_l x1c  \<le> \<Down> Id (unit_propagation_outer_loop_l x1a)\<close>
+    if \<open>(x1c, x1a) \<in> Id\<close>
+    for x1c x1a
+    using that by auto
+  have [refine0]: \<open>cdcl_twl_o_prog_l x1c  \<le> \<Down> Id (cdcl_twl_o_prog_l x1a)\<close>
+    if \<open>(x1c, x1a) \<in> Id\<close>
+    for x1c x1a
+    using that by auto
+  show ?thesis
+    unfolding cdcl_twl_stgy_restart_prog_l_def cdcl_twl_stgy_restart_prog_def uncurry_def
+      cdcl_twl_stgy_restart_abs_l_def
+    apply (intro frefI nres_relI)
+    apply (refine_rcg WHILEIT_refine[where R = \<open>{((brk :: bool, S, n :: nat), (brk', S', n')).
+        (S, S') \<in> Id \<and> brk = brk' \<and> n = n'}\<close>]
+        unit_propagation_outer_loop_l_spec[THEN fref_to_Down]
+        cdcl_twl_o_prog_l_spec[THEN fref_to_Down]
+        restart_abs_l_restart_prog[THEN fref_to_Down_curry2]
+        restart_prog_l_restart_abs_l[THEN fref_to_Down_curry2])
+    subgoal by auto
+    subgoal for x y xa x' x1 x2 x1a x2a
+      by fastforce
+    subgoal by auto
+    subgoal
+      by (simp add: twl_st)
+    subgoal by (auto simp: twl_st)
+    subgoal
+       unfolding cdcl_twl_stgy_restart_prog_inv_def cdcl_twl_stgy_restart_abs_l_inv_def
+       by (auto simp: twl_st)
+    subgoal by auto
+    done
+qed
+
+
+lemma cdcl_twl_stgy_restart_abs_l_cdcl_twl_stgy_restart_abs_l:
+  \<open>(cdcl_twl_stgy_restart_abs_l, cdcl_twl_stgy_restart_prog) \<in>
+     {(S, S'). (S, S') \<in> twl_st_l None \<and> twl_list_invs S \<and>
+       clauses_to_update_l S  = {#}} \<rightarrow>\<^sub>f
+      \<langle>{(S, S'). (S, S') \<in> twl_st_l None \<and> twl_list_invs S}\<rangle> nres_rel\<close>
+  unfolding cdcl_twl_stgy_restart_abs_l_def cdcl_twl_stgy_restart_prog_def uncurry_def
+  apply (intro frefI nres_relI)
+  apply (refine_rcg WHILEIT_refine[where R = \<open>{((brk :: bool, S, n :: nat), (brk', S', n')).
+      (S, S') \<in> twl_st_l None \<and> twl_list_invs S \<and> brk = brk' \<and> n = n' \<and>
+        clauses_to_update_l S = {#}}\<close>]
+      unit_propagation_outer_loop_l_spec[THEN fref_to_Down]
+      cdcl_twl_o_prog_l_spec[THEN fref_to_Down]
+      restart_abs_l_restart_prog[THEN fref_to_Down_curry2])
+  subgoal by simp
+  subgoal for x y xa x' x1 x2 x1a x2a
+    unfolding cdcl_twl_stgy_restart_abs_l_inv_def
+    apply (rule_tac x=y in exI)
+    apply (rule_tac x=\<open>fst (snd x')\<close> in exI)
+    by auto
+  subgoal by fast
+  subgoal
+    unfolding cdcl_twl_stgy_restart_prog_inv_def
+      cdcl_twl_stgy_restart_abs_l_inv_def
+    apply (simp only: prod.case)
+    apply (normalize_goal)+
+    by (simp add: twl_st_l twl_st)
+  subgoal by (auto simp: twl_st_l twl_st)
+  subgoal by auto
+  subgoal by auto
+  subgoal by auto
+ oops
+
+
+lemma (in twl_restart) cdcl_twl_stgy_restart_prog_l_cdcl_twl_stgy_restart_prog:
+  \<open>(cdcl_twl_stgy_restart_prog_l, cdcl_twl_stgy_restart_prog)
+    \<in> {(S, S'). (S, S') \<in> twl_st_l None \<and> twl_list_invs S \<and> clauses_to_update_l S = {#}} \<rightarrow>\<^sub>f
+      \<langle>{(S, S'). (S, S') \<in> twl_st_l None \<and> twl_list_invs S}\<rangle>nres_rel\<close>
+  apply (intro frefI nres_relI)
+  apply (rule order_trans)
+  defer
+  apply (rule cdcl_twl_stgy_restart_abs_l_cdcl_twl_stgy_restart_abs_l[THEN fref_to_Down])
+    apply fast
+    apply assumption
+  apply (rule cdcl_twl_stgy_restart_prog_l_cdcl_twl_stgy_restart_abs_l[THEN fref_to_Down,
     simplified])
   apply simp
   done
